seiostar/RQ.Metaprogram.fst
@@ -371,15 +371,11 @@ let rec create_derivation g (dbmap:db_mapping) (prior_derivs:prior_derivations) 
   | _ -> fail ("not implemented in expressions: " ^ tag_of qfs)
 
 let prove_equality () : Tac unit =
-  explode ();
-  iterAll (fun () ->
-    ignore (trytac (fun () ->
-      or_else trivial trefl)));
-//   iterAll (fun () ->
-//     ignore (trytac simplify_stack_ops);
-//     ignore (trytac (fun () ->
-//       or_else trivial trefl)));
+  ignore (repeat forall_intro);
+  ignore (trytac (fun () ->
+    or_else trivial trefl));
   or_else qed (fun () -> dump "RQ's unification failed"; fail "unification failed")
+
 
 let type_check_derivation g (qderivation:term) (desired_qtyp:term) (unfold_names:list string)  : Tac (r:(term & term){tot_typing g (fst r) (snd r)}) =
   set_guard_policy Goal;
@@ -388,10 +384,10 @@ let type_check_derivation g (qderivation:term) (desired_qtyp:term) (unfold_names
   if List.length l > 0 then fail "Not all implicits solved" else ();
 
   print_debug ("DEBUG: deriv = " ^ term_to_string qderivation);
-  let qderivation' = norm_well_typed_term g [(*delta_only unfold_names;*) delta_only qType_defs_list; iota] qderivation in
-  print_debug ("DEBUG: deriv' = " ^ term_to_string qderivation');
- // let desired_qtyp' = norm_well_typed_term g [delta_only unfold_names; delta_only qType_defs_list; iota] desired_qtyp in
-  let token = must <| core_check_term g qderivation' desired_qtyp E_Total in
+  let qderivation = norm_well_typed_term g [(*delta_only unfold_names;*) delta_only qType_defs_list; iota] qderivation in
+ // print_debug ("DEBUG: deriv' = " ^ term_to_string qderivation');
+  let desired_qtyp' = norm_well_typed_term g [delta_only qType_defs_list; iota] desired_qtyp in
+  let token = must <| core_check_term g qderivation desired_qtyp' E_Total in
 
   print_debug ("DEBUG: core_checm_term successfull, "^ string_of_int (ngoals ()) ^" goals to prove");
   (match ngoals () with
@@ -400,7 +396,8 @@ let type_check_derivation g (qderivation:term) (desired_qtyp:term) (unfold_names
   | _ -> fail "too many goals");
   print_debug ("DEBUG: proved equality!");
   set_guard_policy Force;
-  assume (tot_typing g qderivation desired_qtyp);
+  lem_retype_token g qderivation desired_qtyp' desired_qtyp;
+  token_as_typing g qderivation E_Total desired_qtyp;
   (qderivation, desired_qtyp)
 
 let initial_unfold_fuel : int = 32
