seiostar/RQ.TypingRelation.fst
@@ -232,17 +232,29 @@ let fs_oval_helper #a x pre = fs_oval_helper_g empty #a x pre
 let packed_turnstile_g g (a:qType) (x:fs_val a) =
   pre:spec_env g & (g ⊢ (fs_oval_helper_g g x pre))
 
-let pack_turnstile_g #g #a #x (#pre:spec_env g) (turnstile:(g ⊢ (fs_oval_helper_g g x pre))) :
-  packed_turnstile_g g a x
-   =
-  (| _, turnstile |)
+let pack_turnstile_g
+  (#g:typ_env)
+  (#a:qType)
+  (#x:fs_val a)
+  (#pre:spec_env g)
+  (#x':fs_oval g a pre)
+  (t:typing g x')
+  : Pure (packed_turnstile_g g a x)
+    (requires (x' == (fun _ -> x))) (ensures (fun _ -> True))
+  = (| pre, t |)
 
 let (⊩) (a:qType) (x: fs_val a) =
   packed_turnstile_g empty a x
 
-let pack_turnstile #a #x (#pre:spec_env empty) (turnstile:(empty ⊢ (fs_oval_helper_g empty x pre)))
-  : a ⊩ x =
-  pack_turnstile_g turnstile
+let pack_turnstile
+  (#a:qType)
+  (#x:fs_val a)
+  (#pre:spec_env empty)
+  (#x':fs_oval empty a pre)
+  (t:typing empty x')
+  : Pure (a ⊩ x) (requires (x' == (fun _ -> x))) (ensures (fun _ -> True))
+   =
+  pack_turnstile_g t
 
 let (⊫) (a:qType) (x: fs_val a) =
   pre:spec_env empty &
